Loom/Instances/Rand.lean
@@ -6,31 +6,31 @@ import Plausible.Testable
 
 open Lean.Order Loom
 
-instance (priority := high) {σ : Type} {m : Type → Type v} [Monad m] [LawfulMonad m] [WPMonad m Prop e] [Inhabited σ] :
-  WPMonad (StateT σ m) Prop e where
-  wp x post epost := ∀ s, WPMonad.wp (m := m) (x s) (post ·.1) epost
-  wp_pure x post epost := by simp [pure, StateT.pure, WPMonad.wp_pure (m := m)]
+instance (priority := high) {σ : Type} {m : Type → Type v} [Monad m] [LawfulMonad m] [WP m Prop e] [Inhabited σ] :
+  WP (StateT σ m) Prop e where
+  wp x post epost := ∀ s, WP.wp (m := m) (x s) (post ·.1) epost
+  wp_pure x post epost := by simp [pure, StateT.pure, WP.wp_pure (m := m)]
   wp_bind x f post epost := by
-    intro wph s; apply WPMonad.wp_bind (m := m)
-    apply WPMonad.wp_cons (m := m); rotate_left; apply wph
+    intro wph s; apply WP.wp_bind (m := m)
+    apply WP.wp_cons (m := m); rotate_left; apply wph
     intro x h; simp_all
   wp_cons x post post' epost h := by
-    intro s s'; apply WPMonad.wp_cons (m := m);
+    intro s s'; apply WP.wp_cons (m := m);
     intro x; apply h; solve_by_elim
 
-instance (priority := high) [Monad m] [LawfulMonad m] [WPMonad m Prop e] [Inhabited ρ] :
-  WPMonad (ReaderT ρ m) Prop e where
-  wp x post epost := ∀ r, WPMonad.wp (m := m) (x r) (post ·) epost
-  wp_pure x post epost := by simp [pure, ReaderT.pure, WPMonad.wp_pure (m := m)]
+instance (priority := high) [Monad m] [LawfulMonad m] [WP m Prop e] [Inhabited ρ] :
+  WP (ReaderT ρ m) Prop e where
+  wp x post epost := ∀ r, WP.wp (m := m) (x r) (post ·) epost
+  wp_pure x post epost := by simp [pure, ReaderT.pure, WP.wp_pure (m := m)]
   wp_bind x f post epost := by
-    intro wph r; apply WPMonad.wp_bind (m := m)
-    apply WPMonad.wp_cons (m := m); rotate_left; apply wph
+    intro wph r; apply WP.wp_bind (m := m)
+    apply WP.wp_cons (m := m); rotate_left; apply wph
     intro x h; simp_all
   wp_cons x post post' epost h := by
-    intro r r'; apply WPMonad.wp_cons (m := m);
+    intro r r'; apply WP.wp_cons (m := m);
     intro x; apply h; solve_by_elim
 
-instance (priority := high) : WPMonad (Except ε) Prop PUnit where
+instance (priority := high) : WP (Except ε) Prop PUnit where
   wp x post epost := match x with
     | .ok x => post x
     | .error e => False
@@ -52,11 +52,11 @@ theorem chooseAny_wp (post : α → Prop) [Random Id α] :
 theorem Testable.run_wp [Testable p] c m :
   Triple (p ∧ post) (Testable.runPropE p c m) (fun _ => post) ⟨⟩ := by
   rw [Triple.iff]; intro ⟨ph, posth⟩
-  simp [Testable.runPropE]; apply WPMonad.wp_bind (m := Gen)
+  simp [Testable.runPropE]; apply WP.wp_bind (m := Gen)
   simp [tryCatch, MonadExceptOf.tryCatch, tryCatchThe, Except.tryCatch]
   intro s r; simp
   split
   { simp [wp]; intro s r; split; solve_by_elim
     rename_i a _ _ _ _
     rcases a with ⟨⟨⟩, _⟩ <;> try simp_all [Functor.map, StateT.map, pure, StateT.pure, Except.pure, ReaderT.pure] }
-  erw [WPMonad.wp_pure]; simp; solve_by_elim
+  erw [WP.wp_pure]; simp; solve_by_elim
