Loom/Triple/SpecLemmas.lean
@@ -13,11 +13,10 @@ namespace Loom
 open Lean.Order WP
 
 universe u v
-variable {m : Type u → Type v} {l : Type u} {e : Type u} [CompleteLattice l]
+variable {m : Type u → Type v} {l : Type u} {e : Type u}
+  [Monad m] [CompleteLattice l] [CompleteLattice e] [WP m l e]
 
 /-! # `Monad` -/
-
-variable [Monad m] [WPMonad m l e]
 
 /-- Spec for `pure`: if the precondition entails the postcondition applied to `a`, then `pure a`
 satisfies the triple. -/
@@ -52,7 +51,7 @@ satisfies `post`. -/
 theorem Spec.map' (f : α → β) (x : m α)
     (h : Triple pre x (fun a => post (f a)) epost) :
     Triple pre (f <$> x) post epost :=
-  Triple.iff.mpr (PartialOrder.rel_trans (Triple.iff.mp h) (WPMonad.wp_map f x post epost))
+  Triple.iff.mpr (PartialOrder.rel_trans (Triple.iff.mp h) (WP.wp_map f x post epost))
 
 /-- Canonical spec for `map`: the weakest precondition for `f <$> x` is
 `wp x (fun a => post (f a)) epost`. -/
@@ -65,7 +64,7 @@ then `x <*> y` satisfies `post`. -/
 theorem Spec.seq' (x : m (α → β)) (y : m α)
     (h : Triple pre x (fun f => wp y (fun a => post (f a)) epost) epost) :
     Triple pre (x <*> y) post epost :=
-  Triple.iff.mpr (PartialOrder.rel_trans (Triple.iff.mp h) (WPMonad.wp_seq x y post epost))
+  Triple.iff.mpr (PartialOrder.rel_trans (Triple.iff.mp h) (WP.wp_seq x y post epost))
 
 /-- Canonical spec for `seq`. -/
 theorem Spec.seq (x : m (α → β)) (y : m α) :
@@ -144,7 +143,7 @@ theorem Spec.liftWith_StateT
     (f : (∀{β}, StateT σ m β → m (β × σ)) → m α) (post : α → σ → l) :
     Triple (fun s => wp (f (fun x => x.run s)) (fun a => post a s) epost)
       (MonadControl.liftWith (m:=m) f : StateT σ m α) post epost :=
-  Triple.iff.mpr (by intro s; simp [liftWith_StateT_wp f]; apply WPMonad.wp_map'; ext; rfl)
+  Triple.iff.mpr (by intro s; simp [liftWith_StateT_wp f]; apply WP.wp_map'; ext; rfl)
 
 /-- Spec for `liftWith` on `ReaderT`. -/
 theorem Spec.liftWith_ReaderT
@@ -158,7 +157,7 @@ theorem Spec.liftWith_ExceptT
     (f : (∀{β}, ExceptT ε m β → m (Except ε β)) → m α) (post : α → l) (epost : e × (ε → l)) :
     Triple (wp (f (fun x => x.run)) post epost.1)
       (MonadControl.liftWith (m:=m) f : ExceptT ε m α) post epost :=
-  Triple.iff.mpr (by simp [liftWith_ExceptT_wp f]; apply WPMonad.wp_map'; ext; rfl)
+  Triple.iff.mpr (by simp [liftWith_ExceptT_wp f]; apply WP.wp_map'; ext; rfl)
 
 /-
 /-- Spec for `liftWith` on `OptionT`. -/
@@ -431,7 +430,7 @@ theorem Spec.throw_ExceptT_lift [MonadExceptOf ε m] (err : ε) (post : α → l
     Triple (wp (MonadExceptOf.throw (ε:=ε) err : m (@Except.{u, u} ε' α))
         (fun r => match r with | .ok a => post a | .error e => epost.2 e) epost.1)
       (MonadExceptOf.throw (ε:=ε) err : ExceptT ε' m α) post epost :=
-  Triple.iff.mpr (by rw [throw_lift_ExceptT_wp]; apply WPMonad.wp_cons; intro r; cases r <;> rfl)
+  Triple.iff.mpr (by rw [throw_lift_ExceptT_wp]; apply WP.wp_cons; intro r; cases r <;> rfl)
 
 /-
 /-- Spec for `throw` lifted through `OptionT`. -/
@@ -439,7 +438,7 @@ theorem Spec.throw_Option_lift [MonadExceptOf ε m] (err : ε) (post : α → l)
     Triple (wp (MonadExceptOf.throw (ε:=ε) err : m (Option α))
         (fun | some a => post a | none => epost.2) epost.1)
       (MonadExceptOf.throw (ε:=ε) err : OptionT m α) post epost :=
-  Triple.iff.mpr (by rw [throw_lift_OptionT_wp]; apply WPMonad.wp_cons; intro r; cases r <;> rfl)
+  Triple.iff.mpr (by rw [throw_lift_OptionT_wp]; apply WP.wp_cons; intro r; cases r <;> rfl)
 -/
 
 /-- Spec for `tryCatch` lifted through `ReaderT`. -/
@@ -464,7 +463,7 @@ theorem Spec.tryCatch_ExceptT_lift [MonadExceptOf ε m] (x : ExceptT ε' m α) (
     Triple (wp (MonadExceptOf.tryCatch (ε:=ε) x h : m (@Except.{u, u} ε' α))
         (fun | .ok a => post a | .error e => epost.2 e) epost.1)
       (MonadExceptOf.tryCatch (ε:=ε) x h : ExceptT ε' m α) post epost :=
-  Triple.iff.mpr (by rw [tryCatch_lift_ExceptT_wp]; apply WPMonad.wp_cons; intro r; cases r <;> rfl)
+  Triple.iff.mpr (by rw [tryCatch_lift_ExceptT_wp]; apply WP.wp_cons; intro r; cases r <;> rfl)
 
 /-
 /-- Spec for `tryCatch` lifted through `OptionT`. -/
@@ -473,7 +472,7 @@ theorem Spec.tryCatch_OptionT_lift [MonadExceptOf ε m] (x : OptionT m α) (h : 
     Triple (wp (MonadExceptOf.tryCatch (ε:=ε) x h : m (Option α))
         (fun | some a => post a | none => epost.2) epost.1)
       (MonadExceptOf.tryCatch (ε:=ε) x h : OptionT m α) post epost :=
-  Triple.iff.mpr (by rw [tryCatch_lift_OptionT_wp]; apply WPMonad.wp_cons; intro r; cases r <;> rfl)
+  Triple.iff.mpr (by rw [tryCatch_lift_OptionT_wp]; apply WP.wp_cons; intro r; cases r <;> rfl)
 -/
 
 /-! # `MonadFunctorT` / `MonadControlT` transitivity -/
@@ -520,7 +519,7 @@ open Lean.Order WP
 universe u₁ u₂ v
 
 variable {α : Type u₁} {β : Type (max u₁ u₂)} {m : Type (max u₁ u₂) → Type v} {l : Type (max u₁ u₂)} {e : Type (max u₁ u₂)} [CompleteLattice l]
-variable [Monad m] [WPMonad m l e]
+variable [Monad m] [WP m l e]
 
 /--
 The type of loop invariants used by the specifications of `for ... in ...` loops.
@@ -669,7 +668,7 @@ theorem Spec.foldlM_list_const_inv [LawfulMonad m]
 
 /-- Spec for `forIn'` over a `Std.Legacy.Range` with a loop invariant. -/
 theorem Spec.forIn'_range {β : Type u} {m : Type u → Type v} {l : Type u} {e : Type u}
-    [CompleteLattice l] [Monad m] [WPMonad m l e]
+    [CompleteLattice l] [Monad m] [WP m l e]
     {xs : Std.Legacy.Range} {init : β} {f : (a : Nat) → a ∈ xs → β → m (ForInStep β)}
     (inv : Invariant xs.toList β l)
     (eInv : e)
@@ -691,7 +690,7 @@ theorem Spec.forIn'_range {β : Type u} {m : Type u → Type v} {l : Type u} {e 
 
 /-- Spec for `forIn` over a `Std.Legacy.Range` with a loop invariant. -/
 theorem Spec.forIn_range {β : Type u} {m : Type u → Type v} {l : Type u} {e : Type u}
-    [CompleteLattice l] [Monad m] [WPMonad m l e]
+    [CompleteLattice l] [Monad m] [WP m l e]
     {xs : Std.Legacy.Range} {init : β} {f : Nat → β → m (ForInStep β)}
     (inv : Invariant xs.toList β l)
     (eInv : e)
@@ -714,7 +713,7 @@ theorem Spec.forIn_range {β : Type u} {m : Type u → Type v} {l : Type u} {e :
 open Std Std.PRange in
 /-- Spec for `forIn'` over a `Rcc` range with a loop invariant. -/
 theorem Spec.forIn'_rcc {α β : Type u} {m : Type u → Type v} {l : Type u} {e : Type u}
-    [CompleteLattice l] [Monad m] [WPMonad m l e] [LawfulMonad m]
+    [CompleteLattice l] [Monad m] [WP m l e] [LawfulMonad m]
     [LE α] [DecidableLE α] [UpwardEnumerable α] [Rxc.IsAlwaysFinite α]
     [LawfulUpwardEnumerable α] [LawfulUpwardEnumerableLE α]
     {xs : Rcc α} {init : β} {f : (a : α) → a ∈ xs → β → m (ForInStep β)}
@@ -739,7 +738,7 @@ theorem Spec.forIn'_rcc {α β : Type u} {m : Type u → Type v} {l : Type u} {e
 open Std Std.PRange in
 /-- Spec for `forIn` over a `Rcc` range with a loop invariant. -/
 theorem Spec.forIn_rcc {α β : Type u} {m : Type u → Type v} {l : Type u} {e : Type u}
-    [CompleteLattice l] [Monad m] [WPMonad m l e] [LawfulMonad m]
+    [CompleteLattice l] [Monad m] [WP m l e] [LawfulMonad m]
     [LE α] [DecidableLE α] [UpwardEnumerable α] [Rxc.IsAlwaysFinite α]
     [LawfulUpwardEnumerable α] [LawfulUpwardEnumerableLE α]
     {xs : Rcc α} {init : β} {f : α → β → m (ForInStep β)}
@@ -764,7 +763,7 @@ theorem Spec.forIn_rcc {α β : Type u} {m : Type u → Type v} {l : Type u} {e 
 open Std Std.PRange in
 /-- Spec for `forIn'` over a `Rco` range with a loop invariant. -/
 theorem Spec.forIn'_rco {α β : Type u} {m : Type u → Type v} {l : Type u} {e : Type u}
-    [CompleteLattice l] [Monad m] [WPMonad m l e] [LawfulMonad m]
+    [CompleteLattice l] [Monad m] [WP m l e] [LawfulMonad m]
     [LE α] [LT α] [DecidableLT α] [UpwardEnumerable α] [Rxo.IsAlwaysFinite α]
     [LawfulUpwardEnumerable α] [LawfulUpwardEnumerableLE α] [LawfulUpwardEnumerableLT α]
     {xs : Rco α} {init : β} {f : (a : α) → a ∈ xs → β → m (ForInStep β)}
@@ -789,7 +788,7 @@ theorem Spec.forIn'_rco {α β : Type u} {m : Type u → Type v} {l : Type u} {e
 open Std Std.PRange in
 /-- Spec for `forIn` over a `Rco` range with a loop invariant. -/
 theorem Spec.forIn_rco {α β : Type u} {m : Type u → Type v} {l : Type u} {e : Type u}
-    [CompleteLattice l] [Monad m] [WPMonad m l e] [LawfulMonad m]
+    [CompleteLattice l] [Monad m] [WP m l e] [LawfulMonad m]
     [LE α] [LT α] [DecidableLT α] [UpwardEnumerable α] [Rxo.IsAlwaysFinite α]
     [LawfulUpwardEnumerable α] [LawfulUpwardEnumerableLE α] [LawfulUpwardEnumerableLT α]
     {xs : Rco α} {init : β} {f : α → β → m (ForInStep β)}
@@ -814,7 +813,7 @@ theorem Spec.forIn_rco {α β : Type u} {m : Type u → Type v} {l : Type u} {e 
 open Std Std.PRange in
 /-- Spec for `forIn'` over a `Rci` range with a loop invariant. -/
 theorem Spec.forIn'_rci {α β : Type u} {m : Type u → Type v} {l : Type u} {e : Type u}
-    [CompleteLattice l] [Monad m] [WPMonad m l e] [LawfulMonad m]
+    [CompleteLattice l] [Monad m] [WP m l e] [LawfulMonad m]
     [LE α] [UpwardEnumerable α] [Rxi.IsAlwaysFinite α]
     [LawfulUpwardEnumerable α] [LawfulUpwardEnumerableLE α]
     {xs : Rci α} {init : β} {f : (a : α) → a ∈ xs → β → m (ForInStep β)}
@@ -839,7 +838,7 @@ theorem Spec.forIn'_rci {α β : Type u} {m : Type u → Type v} {l : Type u} {e
 open Std Std.PRange in
 /-- Spec for `forIn` over a `Rci` range with a loop invariant. -/
 theorem Spec.forIn_rci {α β : Type u} {m : Type u → Type v} {l : Type u} {e : Type u}
-    [CompleteLattice l] [Monad m] [WPMonad m l e] [LawfulMonad m]
+    [CompleteLattice l] [Monad m] [WP m l e] [LawfulMonad m]
     [LE α] [UpwardEnumerable α] [Rxi.IsAlwaysFinite α]
     [LawfulUpwardEnumerable α] [LawfulUpwardEnumerableLE α]
     {xs : Rci α} {init : β} {f : α → β → m (ForInStep β)}
@@ -864,7 +863,7 @@ theorem Spec.forIn_rci {α β : Type u} {m : Type u → Type v} {l : Type u} {e 
 open Std Std.PRange in
 /-- Spec for `forIn'` over a `Roc` range with a loop invariant. -/
 theorem Spec.forIn'_roc {α β : Type u} {m : Type u → Type v} {l : Type u} {e : Type u}
-    [CompleteLattice l] [Monad m] [WPMonad m l e] [LawfulMonad m]
+    [CompleteLattice l] [Monad m] [WP m l e] [LawfulMonad m]
     [LE α] [DecidableLE α] [LT α] [UpwardEnumerable α] [Rxc.IsAlwaysFinite α]
     [LawfulUpwardEnumerable α] [LawfulUpwardEnumerableLE α] [LawfulUpwardEnumerableLT α]
     {xs : Roc α} {init : β} {f : (a : α) → a ∈ xs → β → m (ForInStep β)}
@@ -889,7 +888,7 @@ theorem Spec.forIn'_roc {α β : Type u} {m : Type u → Type v} {l : Type u} {e
 open Std Std.PRange in
 /-- Spec for `forIn` over a `Roc` range with a loop invariant. -/
 theorem Spec.forIn_roc {α β : Type u} {m : Type u → Type v} {l : Type u} {e : Type u}
-    [CompleteLattice l] [Monad m] [WPMonad m l e] [LawfulMonad m]
+    [CompleteLattice l] [Monad m] [WP m l e] [LawfulMonad m]
     [LE α] [DecidableLE α] [LT α] [UpwardEnumerable α] [Rxc.IsAlwaysFinite α]
     [LawfulUpwardEnumerable α] [LawfulUpwardEnumerableLE α] [LawfulUpwardEnumerableLT α]
     {xs : Roc α} {init : β} {f : α → β → m (ForInStep β)}
@@ -914,7 +913,7 @@ theorem Spec.forIn_roc {α β : Type u} {m : Type u → Type v} {l : Type u} {e 
 open Std Std.PRange in
 /-- Spec for `forIn'` over a `Roo` range with a loop invariant. -/
 theorem Spec.forIn'_roo {α β : Type u} {m : Type u → Type v} {l : Type u} {e : Type u}
-    [CompleteLattice l] [Monad m] [WPMonad m l e] [LawfulMonad m]
+    [CompleteLattice l] [Monad m] [WP m l e] [LawfulMonad m]
     [LT α] [DecidableLT α] [UpwardEnumerable α] [Rxo.IsAlwaysFinite α]
     [LawfulUpwardEnumerable α] [LawfulUpwardEnumerableLT α]
     {xs : Roo α} {init : β} {f : (a : α) → a ∈ xs → β → m (ForInStep β)}
@@ -939,7 +938,7 @@ theorem Spec.forIn'_roo {α β : Type u} {m : Type u → Type v} {l : Type u} {e
 open Std Std.PRange in
 /-- Spec for `forIn` over a `Roo` range with a loop invariant. -/
 theorem Spec.forIn_roo {α β : Type u} {m : Type u → Type v} {l : Type u} {e : Type u}
-    [CompleteLattice l] [Monad m] [WPMonad m l e] [LawfulMonad m]
+    [CompleteLattice l] [Monad m] [WP m l e] [LawfulMonad m]
     [LT α] [DecidableLT α] [UpwardEnumerable α] [Rxo.IsAlwaysFinite α]
     [LawfulUpwardEnumerable α] [LawfulUpwardEnumerableLT α]
     {xs : Roo α} {init : β} {f : α → β → m (ForInStep β)}
@@ -964,7 +963,7 @@ theorem Spec.forIn_roo {α β : Type u} {m : Type u → Type v} {l : Type u} {e 
 open Std Std.PRange in
 /-- Spec for `forIn'` over a `Roi` range with a loop invariant. -/
 theorem Spec.forIn'_roi {α β : Type u} {m : Type u → Type v} {l : Type u} {e : Type u}
-    [CompleteLattice l] [Monad m] [WPMonad m l e] [LawfulMonad m]
+    [CompleteLattice l] [Monad m] [WP m l e] [LawfulMonad m]
     [LT α] [DecidableLT α] [UpwardEnumerable α] [Rxi.IsAlwaysFinite α]
     [LawfulUpwardEnumerable α] [LawfulUpwardEnumerableLT α]
     {xs : Roi α} {init : β} {f : (a : α) → a ∈ xs → β → m (ForInStep β)}
@@ -989,7 +988,7 @@ theorem Spec.forIn'_roi {α β : Type u} {m : Type u → Type v} {l : Type u} {e
 open Std Std.PRange in
 /-- Spec for `forIn` over a `Roi` range with a loop invariant. -/
 theorem Spec.forIn_roi {α β : Type u} {m : Type u → Type v} {l : Type u} {e : Type u}
-    [CompleteLattice l] [Monad m] [WPMonad m l e] [LawfulMonad m]
+    [CompleteLattice l] [Monad m] [WP m l e] [LawfulMonad m]
     [LT α] [DecidableLT α] [UpwardEnumerable α] [Rxi.IsAlwaysFinite α]
     [LawfulUpwardEnumerable α] [LawfulUpwardEnumerableLT α]
     {xs : Roi α} {init : β} {f : α → β → m (ForInStep β)}
@@ -1014,7 +1013,7 @@ theorem Spec.forIn_roi {α β : Type u} {m : Type u → Type v} {l : Type u} {e 
 open Std Std.PRange in
 /-- Spec for `forIn'` over a `Ric` range with a loop invariant. -/
 theorem Spec.forIn'_ric {α β : Type u} {m : Type u → Type v} {l : Type u} {e : Type u}
-    [CompleteLattice l] [Monad m] [WPMonad m l e] [LawfulMonad m]
+    [CompleteLattice l] [Monad m] [WP m l e] [LawfulMonad m]
     [Least? α] [LE α] [DecidableLE α] [UpwardEnumerable α] [Rxc.IsAlwaysFinite α]
     [LawfulUpwardEnumerable α] [LawfulUpwardEnumerableLeast? α] [LawfulUpwardEnumerableLE α]
     {xs : Ric α} {init : β} {f : (a : α) → a ∈ xs → β → m (ForInStep β)}
@@ -1039,7 +1038,7 @@ theorem Spec.forIn'_ric {α β : Type u} {m : Type u → Type v} {l : Type u} {e
 open Std Std.PRange in
 /-- Spec for `forIn` over a `Ric` range with a loop invariant. -/
 theorem Spec.forIn_ric {α β : Type u} {m : Type u → Type v} {l : Type u} {e : Type u}
-    [CompleteLattice l] [Monad m] [WPMonad m l e] [LawfulMonad m]
+    [CompleteLattice l] [Monad m] [WP m l e] [LawfulMonad m]
     [Least? α] [LE α] [DecidableLE α] [UpwardEnumerable α] [Rxc.IsAlwaysFinite α]
     [LawfulUpwardEnumerable α] [LawfulUpwardEnumerableLeast? α] [LawfulUpwardEnumerableLE α]
     {xs : Ric α} {init : β} {f : α → β → m (ForInStep β)}
@@ -1064,7 +1063,7 @@ theorem Spec.forIn_ric {α β : Type u} {m : Type u → Type v} {l : Type u} {e 
 open Std Std.PRange in
 /-- Spec for `forIn'` over a `Rio` range with a loop invariant. -/
 theorem Spec.forIn'_rio {α β : Type u} {m : Type u → Type v} {l : Type u} {e : Type u}
-    [CompleteLattice l] [Monad m] [WPMonad m l e] [LawfulMonad m]
+    [CompleteLattice l] [Monad m] [WP m l e] [LawfulMonad m]
     [Least? α] [LT α] [DecidableLT α] [UpwardEnumerable α] [Rxo.IsAlwaysFinite α]
     [LawfulUpwardEnumerable α] [LawfulUpwardEnumerableLeast? α] [LawfulUpwardEnumerableLT α]
     {xs : Rio α} {init : β} {f : (a : α) → a ∈ xs → β → m (ForInStep β)}
@@ -1089,7 +1088,7 @@ theorem Spec.forIn'_rio {α β : Type u} {m : Type u → Type v} {l : Type u} {e
 open Std Std.PRange in
 /-- Spec for `forIn` over a `Rio` range with a loop invariant. -/
 theorem Spec.forIn_rio {α β : Type u} {m : Type u → Type v} {l : Type u} {e : Type u}
-    [CompleteLattice l] [Monad m] [WPMonad m l e] [LawfulMonad m]
+    [CompleteLattice l] [Monad m] [WP m l e] [LawfulMonad m]
     [Least? α] [LT α] [DecidableLT α] [UpwardEnumerable α] [Rxo.IsAlwaysFinite α]
     [LawfulUpwardEnumerable α] [LawfulUpwardEnumerableLeast? α] [LawfulUpwardEnumerableLT α]
     {xs : Rio α} {init : β} {f : α → β → m (ForInStep β)}
@@ -1114,7 +1113,7 @@ theorem Spec.forIn_rio {α β : Type u} {m : Type u → Type v} {l : Type u} {e 
 open Std Std.PRange in
 /-- Spec for `forIn'` over a `Rii` range with a loop invariant. -/
 theorem Spec.forIn'_rii {α β : Type u} {m : Type u → Type v} {l : Type u} {e : Type u}
-    [CompleteLattice l] [Monad m] [WPMonad m l e] [LawfulMonad m]
+    [CompleteLattice l] [Monad m] [WP m l e] [LawfulMonad m]
     [Least? α] [UpwardEnumerable α] [Rxi.IsAlwaysFinite α]
     [LawfulUpwardEnumerable α] [LawfulUpwardEnumerableLeast? α]
     {xs : Rii α} {init : β} {f : (a : α) → a ∈ xs → β → m (ForInStep β)}
@@ -1139,7 +1138,7 @@ theorem Spec.forIn'_rii {α β : Type u} {m : Type u → Type v} {l : Type u} {e
 open Std Std.PRange in
 /-- Spec for `forIn` over a `Rii` range with a loop invariant. -/
 theorem Spec.forIn_rii {α β : Type u} {m : Type u → Type v} {l : Type u} {e : Type u}
-    [CompleteLattice l] [Monad m] [WPMonad m l e] [LawfulMonad m]
+    [CompleteLattice l] [Monad m] [WP m l e] [LawfulMonad m]
     [Least? α] [UpwardEnumerable α] [Rxi.IsAlwaysFinite α]
     [LawfulUpwardEnumerable α] [LawfulUpwardEnumerableLeast? α]
     {xs : Rii α} {init : β} {f : α → β → m (ForInStep β)}
@@ -1164,7 +1163,7 @@ theorem Spec.forIn_rii {α β : Type u} {m : Type u → Type v} {l : Type u} {e 
 open Std Std.Iterators in
 /-- Spec for `forIn` over a `Slice` with a loop invariant. -/
 theorem Spec.forIn_slice {δ : Type u} {m : Type u → Type w} {l : Type u} {e : Type u}
-    [CompleteLattice l] [Monad m] [WPMonad m l e] [LawfulMonad m]
+    [CompleteLattice l] [Monad m] [WP m l e] [LawfulMonad m]
     {γ : Type u'} {α β : Type u}
     [ToIterator (Slice γ) Id α β]
     [Iterator α Id β]
@@ -1193,7 +1192,7 @@ open Std Std.Iterators
 
 /-- Spec for `forIn` over an `Iter` with a loop invariant. -/
 theorem Spec.forIn_iter {α β γ : Type u} {m : Type u → Type w} {l : Type u} {e : Type u}
-    [CompleteLattice l] [Monad m] [WPMonad m l e] [LawfulMonad m]
+    [CompleteLattice l] [Monad m] [WP m l e] [LawfulMonad m]
     [Iterator α Id β] [Finite α Id] [IteratorLoop α Id m] [LawfulIteratorLoop α Id m]
     {init : γ} {f : β → γ → m (ForInStep γ)}
     {it : Iter (α := α) β}
@@ -1214,7 +1213,7 @@ theorem Spec.forIn_iter {α β γ : Type u} {m : Type u → Type w} {l : Type u}
 
 /-- Spec for `forIn` over an `IterM Id` with a loop invariant. -/
 theorem Spec.forIn_iterM_id {α β γ : Type u} {m : Type u → Type w} {l : Type u} {e : Type u}
-    [CompleteLattice l] [Monad m] [WPMonad m l e] [LawfulMonad m]
+    [CompleteLattice l] [Monad m] [WP m l e] [LawfulMonad m]
     [Iterator α Id β] [Finite α Id] [IteratorLoop α Id m] [LawfulIteratorLoop α Id m]
     {init : γ} {f : β → γ → m (ForInStep γ)}
     {it : IterM (α := α) Id β}
@@ -1237,7 +1236,7 @@ theorem Spec.forIn_iterM_id {α β γ : Type u} {m : Type u → Type w} {l : Typ
 
 /-- Spec for `Iter.foldM` with a loop invariant. -/
 theorem Spec.foldM_iter {α β γ : Type u} {m : Type u → Type w} {l : Type u} {e : Type u}
-    [CompleteLattice l] [Monad m] [WPMonad m l e] [LawfulMonad m]
+    [CompleteLattice l] [Monad m] [WP m l e] [LawfulMonad m]
     [Iterator α Id β] [Finite α Id] [IteratorLoop α Id m] [LawfulIteratorLoop α Id m]
     {it : Iter (α := α) β}
     {init : γ} {f : γ → β → m γ}
@@ -1256,7 +1255,7 @@ theorem Spec.foldM_iter {α β γ : Type u} {m : Type u → Type w} {l : Type u}
 
 /-- Spec for `IterM.foldM` over an `IterM Id` with a loop invariant. -/
 theorem Spec.foldM_iterM_id {α β γ : Type u} {m : Type u → Type w} {l : Type u} {e : Type u}
-    [CompleteLattice l] [Monad m] [WPMonad m l e] [LawfulMonad m]
+    [CompleteLattice l] [Monad m] [WP m l e] [LawfulMonad m]
     [Iterator α Id β] [Finite α Id] [IteratorLoop α Id m] [LawfulIteratorLoop α Id m]
     {it : IterM (α := α) Id β}
     {init : γ} {f : γ → β → m γ}
@@ -1276,7 +1275,7 @@ theorem Spec.foldM_iterM_id {α β γ : Type u} {m : Type u → Type w} {l : Typ
 theorem Spec.IterM.forIn_filterMapWithPostcondition {α β β₂ γ : Type w}
     {m : Type w → Type w'} {n : Type w → Type w''} {o : Type w → Type w'''}
     {l : Type w} {e : Type w} [CompleteLattice l]
-    [Monad m] [LawfulMonad m] [Monad n] [LawfulMonad n] [Monad o] [LawfulMonad o] [WPMonad o l e]
+    [Monad m] [LawfulMonad m] [Monad n] [LawfulMonad n] [Monad o] [LawfulMonad o] [WP o l e]
     [MonadLiftT m n] [LawfulMonadLiftT m n] [MonadLiftT n o] [LawfulMonadLiftT n o]
     [Iterator α m β] [Finite α m]
     [IteratorLoop α m o] [LawfulIteratorLoop α m o]
@@ -1294,7 +1293,7 @@ theorem Spec.IterM.forIn_filterMapWithPostcondition {α β β₂ γ : Type w}
 theorem Spec.IterM.forIn_filterMapM {α β β₂ γ : Type w}
     {m : Type w → Type w'} {n : Type w → Type w''} {o : Type w → Type w'''}
     {l : Type w} {e : Type w} [CompleteLattice l]
-    [Monad m] [LawfulMonad m] [Monad n] [LawfulMonad n] [Monad o] [LawfulMonad o] [WPMonad o l e]
+    [Monad m] [LawfulMonad m] [Monad n] [LawfulMonad n] [Monad o] [LawfulMonad o] [WP o l e]
     [MonadAttach n] [WeaklyLawfulMonadAttach n]
     [MonadLiftT m n] [LawfulMonadLiftT m n] [MonadLiftT n o] [LawfulMonadLiftT n o]
     [Iterator α m β] [Finite α m]
@@ -1313,7 +1312,7 @@ theorem Spec.IterM.forIn_filterMapM {α β β₂ γ : Type w}
 theorem Spec.IterM.forIn_filterMap {α β β₂ γ : Type w}
     {m : Type w → Type w'} {n : Type w → Type w''}
     {l : Type w} {e : Type w} [CompleteLattice l]
-    [Monad m] [LawfulMonad m] [Monad n] [LawfulMonad n] [WPMonad n l e]
+    [Monad m] [LawfulMonad m] [Monad n] [LawfulMonad n] [WP n l e]
     [MonadLiftT m n] [LawfulMonadLiftT m n]
     [Iterator α m β] [Finite α m]
     [IteratorLoop α m n] [LawfulIteratorLoop α m n]
@@ -1329,7 +1328,7 @@ theorem Spec.IterM.forIn_filterMap {α β β₂ γ : Type w}
 theorem Spec.IterM.forIn_mapWithPostcondition {α β β₂ γ : Type w}
     {m : Type w → Type w'} {n : Type w → Type w''} {o : Type w → Type w'''}
     {l : Type w} {e : Type w} [CompleteLattice l]
-    [Monad m] [LawfulMonad m] [Monad n] [LawfulMonad n] [Monad o] [LawfulMonad o] [WPMonad o l e]
+    [Monad m] [LawfulMonad m] [Monad n] [LawfulMonad n] [Monad o] [LawfulMonad o] [WP o l e]
     [MonadLiftT m n] [LawfulMonadLiftT m n] [MonadLiftT n o] [LawfulMonadLiftT n o]
     [Iterator α m β] [Finite α m]
     [IteratorLoop α m o] [LawfulIteratorLoop α m o]
@@ -1344,7 +1343,7 @@ theorem Spec.IterM.forIn_mapWithPostcondition {α β β₂ γ : Type w}
 theorem Spec.IterM.forIn_mapM {α β β₂ γ : Type w}
     {m : Type w → Type w'} {n : Type w → Type w''} {o : Type w → Type w'''}
     {l : Type w} {e : Type w} [CompleteLattice l]
-    [Monad m] [LawfulMonad m] [Monad n] [LawfulMonad n] [Monad o] [LawfulMonad o] [WPMonad o l e]
+    [Monad m] [LawfulMonad m] [Monad n] [LawfulMonad n] [Monad o] [LawfulMonad o] [WP o l e]
     [MonadAttach n] [WeaklyLawfulMonadAttach n]
     [MonadLiftT m n] [LawfulMonadLiftT m n] [MonadLiftT n o] [LawfulMonadLiftT n o]
     [Iterator α m β] [Finite α m]
@@ -1360,7 +1359,7 @@ theorem Spec.IterM.forIn_mapM {α β β₂ γ : Type w}
 theorem Spec.IterM.forIn_map {α β β₂ γ : Type w}
     {m : Type w → Type w'} {n : Type w → Type w''}
     {l : Type w} {e : Type w} [CompleteLattice l]
-    [Monad m] [LawfulMonad m] [Monad n] [LawfulMonad n] [WPMonad n l e]
+    [Monad m] [LawfulMonad m] [Monad n] [LawfulMonad n] [WP n l e]
     [MonadLiftT m n] [LawfulMonadLiftT m n]
     [Iterator α m β] [Finite α m] [IteratorLoop α m n] [LawfulIteratorLoop α m n]
     {it : IterM (α := α) m β} {f : β → β₂} {init : γ} {g : β₂ → γ → n (ForInStep γ)}
@@ -1372,7 +1371,7 @@ theorem Spec.IterM.forIn_map {α β β₂ γ : Type w}
 theorem Spec.IterM.forIn_filterWithPostcondition {α β γ : Type w}
     {m : Type w → Type w'} {n : Type w → Type w''} {o : Type w → Type w'''}
     {l : Type w} {e : Type w} [CompleteLattice l]
-    [Monad m] [LawfulMonad m] [Monad n] [LawfulMonad n] [Monad o] [LawfulMonad o] [WPMonad o l e]
+    [Monad m] [LawfulMonad m] [Monad n] [LawfulMonad n] [Monad o] [LawfulMonad o] [WP o l e]
     [MonadLiftT m n] [LawfulMonadLiftT m n] [MonadLiftT n o] [LawfulMonadLiftT n o]
     [Iterator α m β] [Finite α m]
     [IteratorLoop α m o] [LawfulIteratorLoop α m o]
@@ -1387,7 +1386,7 @@ theorem Spec.IterM.forIn_filterWithPostcondition {α β γ : Type w}
 theorem Spec.IterM.forIn_filterM {α β γ : Type w}
     {m : Type w → Type w'} {n : Type w → Type w''} {o : Type w → Type w'''}
     {l : Type w} {e : Type w} [CompleteLattice l]
-    [Monad m] [LawfulMonad m] [Monad n] [LawfulMonad n] [Monad o] [LawfulMonad o] [WPMonad o l e]
+    [Monad m] [LawfulMonad m] [Monad n] [LawfulMonad n] [Monad o] [LawfulMonad o] [WP o l e]
     [MonadAttach n] [WeaklyLawfulMonadAttach n]
     [MonadLiftT m n] [LawfulMonadLiftT m n] [MonadLiftT n o] [LawfulMonadLiftT n o]
     [Iterator α m β] [Finite α m]
@@ -1403,7 +1402,7 @@ theorem Spec.IterM.forIn_filterM {α β γ : Type w}
 theorem Spec.IterM.forIn_filter {α β γ : Type w}
     {m : Type w → Type w'} {n : Type w → Type w''}
     {l : Type w} {e : Type w} [CompleteLattice l]
-    [Monad m] [LawfulMonad m] [Monad n] [LawfulMonad n] [WPMonad n l e]
+    [Monad m] [LawfulMonad m] [Monad n] [LawfulMonad n] [WP n l e]
     [MonadLiftT m n] [LawfulMonadLiftT m n]
     [Iterator α m β] [Finite α m] [IteratorLoop α m n] [LawfulIteratorLoop α m n]
     {it : IterM (α := α) m β} {f : β → Bool} {init : γ} {g : β → γ → n (ForInStep γ)}
@@ -1416,7 +1415,7 @@ theorem Spec.IterM.foldM_filterMapWithPostcondition {α β γ δ : Type w}
     {m : Type w → Type w'} {n : Type w → Type w''} {o : Type w → Type w'''}
     {l : Type w} {e : Type w} [CompleteLattice l]
     [Iterator α m β] [Finite α m]
-    [Monad m] [Monad n] [Monad o] [LawfulMonad m] [LawfulMonad n] [LawfulMonad o] [WPMonad o l e]
+    [Monad m] [Monad n] [Monad o] [LawfulMonad m] [LawfulMonad n] [LawfulMonad o] [WP o l e]
     [IteratorLoop α m n] [IteratorLoop α m o]
     [LawfulIteratorLoop α m n] [LawfulIteratorLoop α m o]
     [MonadLiftT m n] [MonadLiftT n o] [LawfulMonadLiftT m n] [LawfulMonadLiftT n o]
@@ -1436,7 +1435,7 @@ theorem Spec.IterM.foldM_filterMapM {α β γ δ : Type w}
     [Iterator α m β] [Finite α m]
     [Monad m] [LawfulMonad m]
     [Monad n] [MonadAttach n] [LawfulMonad n] [WeaklyLawfulMonadAttach n]
-    [Monad o] [LawfulMonad o] [WPMonad o l e]
+    [Monad o] [LawfulMonad o] [WP o l e]
     [IteratorLoop α m n] [IteratorLoop α m o]
     [LawfulIteratorLoop α m n] [LawfulIteratorLoop α m o]
     [MonadLiftT m n] [MonadLiftT n o] [LawfulMonadLiftT m n] [LawfulMonadLiftT n o]
@@ -1454,7 +1453,7 @@ theorem Spec.IterM.foldM_mapWithPostcondition {α β γ δ : Type w}
     {m : Type w → Type w'} {n : Type w → Type w''} {o : Type w → Type w'''}
     {l : Type w} {e : Type w} [CompleteLattice l]
     [Iterator α m β] [Finite α m]
-    [Monad m] [Monad n] [Monad o] [LawfulMonad m] [LawfulMonad n] [LawfulMonad o] [WPMonad o l e]
+    [Monad m] [Monad n] [Monad o] [LawfulMonad m] [LawfulMonad n] [LawfulMonad o] [WP o l e]
     [IteratorLoop α m n] [IteratorLoop α m o]
     [LawfulIteratorLoop α m n] [LawfulIteratorLoop α m o]
     [MonadLiftT m n] [MonadLiftT n o] [LawfulMonadLiftT m n] [LawfulMonadLiftT n o]
@@ -1472,7 +1471,7 @@ theorem Spec.IterM.foldM_mapM {α β γ δ : Type w}
     [Iterator α m β] [Finite α m]
     [Monad m] [LawfulMonad m]
     [Monad n] [MonadAttach n] [LawfulMonad n] [WeaklyLawfulMonadAttach n]
-    [Monad o] [LawfulMonad o] [WPMonad o l e]
+    [Monad o] [LawfulMonad o] [WP o l e]
     [IteratorLoop α m n] [IteratorLoop α m o]
     [LawfulIteratorLoop α m n] [LawfulIteratorLoop α m o]
     [MonadLiftT m n] [MonadLiftT n o] [LawfulMonadLiftT m n] [LawfulMonadLiftT n o]
@@ -1488,7 +1487,7 @@ theorem Spec.IterM.foldM_filterWithPostcondition {α β δ : Type w}
     {m : Type w → Type w'} {n : Type w → Type w''} {o : Type w → Type w'''}
     {l : Type w} {e : Type w} [CompleteLattice l]
     [Iterator α m β] [Finite α m]
-    [Monad m] [Monad n] [Monad o] [LawfulMonad m] [LawfulMonad n] [LawfulMonad o] [WPMonad o l e]
+    [Monad m] [Monad n] [Monad o] [LawfulMonad m] [LawfulMonad n] [LawfulMonad o] [WP o l e]
     [IteratorLoop α m n] [IteratorLoop α m o]
     [LawfulIteratorLoop α m n] [LawfulIteratorLoop α m o]
     [MonadLiftT m n] [MonadLiftT n o] [LawfulMonadLiftT m n] [LawfulMonadLiftT n o]
@@ -1506,7 +1505,7 @@ theorem Spec.IterM.foldM_filterM {α β δ : Type w}
     [Iterator α m β] [Finite α m]
     [Monad m] [LawfulMonad m]
     [Monad n] [MonadAttach n] [LawfulMonad n] [WeaklyLawfulMonadAttach n]
-    [Monad o] [LawfulMonad o] [WPMonad o l e]
+    [Monad o] [LawfulMonad o] [WP o l e]
     [IteratorLoop α m n] [IteratorLoop α m o]
     [LawfulIteratorLoop α m n] [LawfulIteratorLoop α m o]
     [MonadLiftT m n] [MonadLiftT n o] [LawfulMonadLiftT m n] [LawfulMonadLiftT n o]
@@ -1521,7 +1520,7 @@ theorem Spec.IterM.foldM_filterM {α β δ : Type w}
 theorem Spec.IterM.foldM_filterMap {α β γ δ : Type w}
     {m : Type w → Type w'} {n : Type w → Type w''}
     {l : Type w} {e : Type w} [CompleteLattice l]
-    [Iterator α m β] [Finite α m] [Monad m] [Monad n] [LawfulMonad m] [LawfulMonad n] [WPMonad n l e]
+    [Iterator α m β] [Finite α m] [Monad m] [Monad n] [LawfulMonad m] [LawfulMonad n] [WP n l e]
     [IteratorLoop α m n]
     [LawfulIteratorLoop α m n]
     [MonadLiftT m n] [LawfulMonadLiftT m n]
@@ -1536,7 +1535,7 @@ theorem Spec.IterM.foldM_filterMap {α β γ δ : Type w}
 theorem Spec.IterM.foldM_map {α β γ δ : Type w}
     {m : Type w → Type w'} {n : Type w → Type w''}
     {l : Type w} {e : Type w} [CompleteLattice l]
-    [Iterator α m β] [Finite α m] [Monad m] [Monad n] [LawfulMonad m] [LawfulMonad n] [WPMonad n l e]
+    [Iterator α m β] [Finite α m] [Monad m] [Monad n] [LawfulMonad m] [LawfulMonad n] [WP n l e]
     [IteratorLoop α m n] [LawfulIteratorLoop α m n]
     [MonadLiftT m n] [LawfulMonadLiftT m n]
     {f : β → γ} {g : δ → γ → n δ} {init : δ} {it : IterM (α := α) m β}
@@ -1548,7 +1547,7 @@ theorem Spec.IterM.foldM_map {α β γ δ : Type w}
 theorem Spec.IterM.foldM_filter {α β δ : Type w}
     {m : Type w → Type w'} {n : Type w → Type w''}
     {l : Type w} {e : Type w} [CompleteLattice l]
-    [Iterator α m β] [Finite α m] [Monad m] [Monad n] [LawfulMonad m] [LawfulMonad n] [WPMonad n l e]
+    [Iterator α m β] [Finite α m] [Monad m] [Monad n] [LawfulMonad m] [LawfulMonad n] [WP n l e]
     [IteratorLoop α m n]
     [LawfulIteratorLoop α m n]
     [MonadLiftT m n] [LawfulMonadLiftT m n]
@@ -1563,7 +1562,7 @@ theorem Spec.IterM.fold_filterMapWithPostcondition {α β γ δ : Type w}
     {l : Type w} {e : Type w} [CompleteLattice l]
     [Iterator α m β] [Finite α m]
     [Monad m] [LawfulMonad m]
-    [Monad n] [LawfulMonad n] [WPMonad n l e]
+    [Monad n] [LawfulMonad n] [WP n l e]
     [IteratorLoop α m n] [LawfulIteratorLoop α m n]
     [MonadLiftT m n] [LawfulMonadLiftT m n]
     {f : β → PostconditionT n (Option γ)} {g : δ → γ → δ} {init : δ} {it : IterM (α := α) m β}
@@ -1579,7 +1578,7 @@ theorem Spec.IterM.fold_filterMapM {α β γ δ : Type w}
     {l : Type w} {e : Type w} [CompleteLattice l]
     [Iterator α m β] [Finite α m]
     [Monad m] [LawfulMonad m]
-    [Monad n] [MonadAttach n] [LawfulMonad n] [WeaklyLawfulMonadAttach n] [WPMonad n l e]
+    [Monad n] [MonadAttach n] [LawfulMonad n] [WeaklyLawfulMonadAttach n] [WP n l e]
     [IteratorLoop α m n] [LawfulIteratorLoop α m n]
     [MonadLiftT m n] [LawfulMonadLiftT m n]
     {f : β → n (Option γ)} {g : δ → γ → δ} {init : δ} {it : IterM (α := α) m β}
@@ -1595,7 +1594,7 @@ theorem Spec.IterM.fold_mapWithPostcondition {α β γ δ : Type w}
     {l : Type w} {e : Type w} [CompleteLattice l]
     [Iterator α m β] [Finite α m]
     [Monad m] [LawfulMonad m]
-    [Monad n] [LawfulMonad n] [WPMonad n l e]
+    [Monad n] [LawfulMonad n] [WP n l e]
     [IteratorLoop α m n] [LawfulIteratorLoop α m n]
     [MonadLiftT m n] [LawfulMonadLiftT m n]
     {f : β → PostconditionT n γ} {g : δ → γ → δ} {init : δ} {it : IterM (α := α) m β}
@@ -1609,7 +1608,7 @@ theorem Spec.IterM.fold_mapM {α β γ δ : Type w}
     {l : Type w} {e : Type w} [CompleteLattice l]
     [Iterator α m β] [Finite α m]
     [Monad m] [LawfulMonad m]
-    [Monad n] [MonadAttach n] [LawfulMonad n] [WeaklyLawfulMonadAttach n] [WPMonad n l e]
+    [Monad n] [MonadAttach n] [LawfulMonad n] [WeaklyLawfulMonadAttach n] [WP n l e]
     [IteratorLoop α m n] [LawfulIteratorLoop α m n]
     [MonadLiftT m n] [LawfulMonadLiftT m n]
     {f : β → n γ} {g : δ → γ → δ} {init : δ} {it : IterM (α := α) m β}
@@ -1623,7 +1622,7 @@ theorem Spec.IterM.fold_filterWithPostcondition {α β δ : Type w}
     {l : Type w} {e : Type w} [CompleteLattice l]
     [Iterator α m β] [Finite α m]
     [Monad m] [LawfulMonad m]
-    [Monad n] [LawfulMonad n] [WPMonad n l e]
+    [Monad n] [LawfulMonad n] [WP n l e]
     [IteratorLoop α m n] [LawfulIteratorLoop α m n]
     [MonadLiftT m n] [LawfulMonadLiftT m n]
     {f : β → PostconditionT n (ULift Bool)} {g : δ → β → δ} {init : δ} {it : IterM (α := α) m β}
@@ -1637,7 +1636,7 @@ theorem Spec.IterM.fold_filterM {α β δ : Type w}
     {l : Type w} {e : Type w} [CompleteLattice l]
     [Iterator α m β] [Finite α m]
     [Monad m] [LawfulMonad m]
-    [Monad n] [MonadAttach n] [LawfulMonad n] [WeaklyLawfulMonadAttach n] [WPMonad n l e]
+    [Monad n] [MonadAttach n] [LawfulMonad n] [WeaklyLawfulMonadAttach n] [WP n l e]
     [IteratorLoop α m n] [LawfulIteratorLoop α m n]
     [MonadLiftT m n] [LawfulMonadLiftT m n]
     {f : β → n (ULift Bool)} {g : δ → β → δ} {init : δ} {it : IterM (α := α) m β}
@@ -1649,7 +1648,7 @@ theorem Spec.IterM.fold_filterM {α β δ : Type w}
 theorem Spec.IterM.fold_filterMap {α β γ δ : Type w}
     {m : Type w → Type w'}
     {l : Type w} {e : Type w} [CompleteLattice l]
-    [Iterator α m β] [Finite α m] [Monad m] [LawfulMonad m] [WPMonad m l e]
+    [Iterator α m β] [Finite α m] [Monad m] [LawfulMonad m] [WP m l e]
     [IteratorLoop α m m] [LawfulIteratorLoop α m m]
     {f : β → Option γ} {g : δ → γ → δ} {init : δ} {it : IterM (α := α) m β}
     {P : l} {Q : δ → l} {eQ : e}
@@ -1663,7 +1662,7 @@ theorem Spec.IterM.fold_filterMap {α β γ δ : Type w}
 theorem Spec.IterM.fold_map {α β γ δ : Type w}
     {m : Type w → Type w'}
     {l : Type w} {e : Type w} [CompleteLattice l]
-    [Iterator α m β] [Finite α m] [Monad m] [LawfulMonad m] [WPMonad m l e]
+    [Iterator α m β] [Finite α m] [Monad m] [LawfulMonad m] [WP m l e]
     [IteratorLoop α m m] [LawfulIteratorLoop α m m]
     {f : β → γ} {g : δ → γ → δ} {init : δ} {it : IterM (α := α) m β}
     {P : l} {Q : δ → l} {eQ : e}
@@ -1674,7 +1673,7 @@ theorem Spec.IterM.fold_map {α β γ δ : Type w}
 theorem Spec.IterM.fold_filter {α β δ : Type w}
     {m : Type w → Type w'}
     {l : Type w} {e : Type w} [CompleteLattice l]
-    [Iterator α m β] [Finite α m] [Monad m] [LawfulMonad m] [WPMonad m l e]
+    [Iterator α m β] [Finite α m] [Monad m] [LawfulMonad m] [WP m l e]
     [IteratorLoop α m m] [LawfulIteratorLoop α m m]
     {f : β → Bool} {g : δ → β → δ} {init : δ} {it : IterM (α := α) m β}
     {P : l} {Q : δ → l} {eQ : e}
@@ -1686,7 +1685,7 @@ theorem Spec.Iter.forIn_filterMapWithPostcondition {α β β₂ γ : Type w}
     {n : Type w → Type w'} {o : Type w → Type w''}
     {l : Type w} {e : Type w} [CompleteLattice l]
     [Iterator α Id β]
-    [Monad n] [LawfulMonad n] [Monad o] [LawfulMonad o] [WPMonad o l e]
+    [Monad n] [LawfulMonad n] [Monad o] [LawfulMonad o] [WP o l e]
     [MonadLiftT n o] [LawfulMonadLiftT n o] [Finite α Id]
     [IteratorLoop α Id o] [LawfulIteratorLoop α Id o]
     {it : Iter (α := α) β} {f : β → PostconditionT n (Option β₂)} {init : γ}
@@ -1702,7 +1701,7 @@ theorem Spec.Iter.forIn_filterMapM {α β β₂ γ : Type w}
     {n : Type w → Type w'} {o : Type w → Type w''}
     {l : Type w} {e : Type w} [CompleteLattice l]
     [Iterator α Id β]
-    [Monad n] [LawfulMonad n] [Monad o] [LawfulMonad o] [WPMonad o l e]
+    [Monad n] [LawfulMonad n] [Monad o] [LawfulMonad o] [WP o l e]
     [MonadAttach n] [WeaklyLawfulMonadAttach n]
     [MonadLiftT n o] [LawfulMonadLiftT n o]
     [Finite α Id] [IteratorLoop α Id o] [LawfulIteratorLoop α Id o]
@@ -1719,7 +1718,7 @@ theorem Spec.Iter.forIn_filterMap {α β β₂ γ : Type w}
     {n : Type w → Type w'}
     {l : Type w} {e : Type w} [CompleteLattice l]
     [Iterator α Id β]
-    [Monad n] [LawfulMonad n] [WPMonad n l e] [Finite α Id]
+    [Monad n] [LawfulMonad n] [WP n l e] [Finite α Id]
     [IteratorLoop α Id n] [LawfulIteratorLoop α Id n]
     {it : Iter (α := α) β} {f : β → Option β₂} {init : γ} {g : β₂ → γ → n (ForInStep γ)}
     {P : l} {Q : γ → l} {eQ : e}
@@ -1734,7 +1733,7 @@ theorem Spec.Iter.forIn_mapWithPostcondition {α β β₂ γ : Type w}
     {n : Type w → Type w'} {o : Type w → Type w''}
     {l : Type w} {e : Type w} [CompleteLattice l]
     [Iterator α Id β]
-    [Monad n] [LawfulMonad n] [Monad o] [LawfulMonad o] [WPMonad o l e]
+    [Monad n] [LawfulMonad n] [Monad o] [LawfulMonad o] [WP o l e]
     [MonadLiftT n o] [LawfulMonadLiftT n o] [Finite α Id]
     [IteratorLoop α Id o] [LawfulIteratorLoop α Id o]
     {it : Iter (α := α) β} {f : β → PostconditionT n β₂} {init : γ}
@@ -1747,7 +1746,7 @@ theorem Spec.Iter.forIn_mapM {α β β₂ γ : Type w}
     {n : Type w → Type w'} {o : Type w → Type w''}
     {l : Type w} {e : Type w} [CompleteLattice l]
     [Iterator α Id β]
-    [Monad n] [LawfulMonad n] [Monad o] [LawfulMonad o] [WPMonad o l e]
+    [Monad n] [LawfulMonad n] [Monad o] [LawfulMonad o] [WP o l e]
     [MonadAttach n] [WeaklyLawfulMonadAttach n]
     [MonadLiftT n o] [LawfulMonadLiftT n o]
     [Finite α Id]
@@ -1762,7 +1761,7 @@ theorem Spec.Iter.forIn_map {α β β₂ γ : Type w}
     {n : Type w → Type w'}
     {l : Type w} {e : Type w} [CompleteLattice l]
     [Iterator α Id β]
-    [Monad n] [LawfulMonad n] [WPMonad n l e]
+    [Monad n] [LawfulMonad n] [WP n l e]
     [Finite α Id] [IteratorLoop α Id n] [LawfulIteratorLoop α Id n]
     {it : Iter (α := α) β} {f : β → β₂} {init : γ} {g : β₂ → γ → n (ForInStep γ)}
     {P : l} {Q : γ → l} {eQ : e}
@@ -1774,7 +1773,7 @@ theorem Spec.Iter.forIn_filterWithPostcondition {α β γ : Type w}
     {n : Type w → Type w'} {o : Type w → Type w''}
     {l : Type w} {e : Type w} [CompleteLattice l]
     [Iterator α Id β]
-    [Monad n] [LawfulMonad n] [Monad o] [LawfulMonad o] [WPMonad o l e]
+    [Monad n] [LawfulMonad n] [Monad o] [LawfulMonad o] [WP o l e]
     [MonadLiftT n o] [LawfulMonadLiftT n o]
     [Finite α Id] [IteratorLoop α Id o] [LawfulIteratorLoop α Id o]
     {it : Iter (α := α) β} {f : β → PostconditionT n (ULift Bool)} {init : γ}
@@ -1787,7 +1786,7 @@ theorem Spec.Iter.forIn_filterM {α β γ : Type w}
     {n : Type w → Type w'} {o : Type w → Type w''}
     {l : Type w} {e : Type w} [CompleteLattice l]
     [Iterator α Id β]
-    [Monad n] [LawfulMonad n] [Monad o] [LawfulMonad o] [WPMonad o l e]
+    [Monad n] [LawfulMonad n] [Monad o] [LawfulMonad o] [WP o l e]
     [MonadAttach n] [WeaklyLawfulMonadAttach n]
     [MonadLiftT n o] [LawfulMonadLiftT n o] [Finite α Id]
     [IteratorLoop α Id o] [LawfulIteratorLoop α Id o]
@@ -1801,7 +1800,7 @@ theorem Spec.Iter.forIn_filter {α β γ : Type w}
     {n : Type w → Type w'}
     {l : Type w} {e : Type w} [CompleteLattice l]
     [Iterator α Id β]
-    [Monad n] [LawfulMonad n] [WPMonad n l e]
+    [Monad n] [LawfulMonad n] [WP n l e]
     [Finite α Id] [IteratorLoop α Id n] [LawfulIteratorLoop α Id n]
     {it : Iter (α := α) β} {f : β → Bool} {init : γ} {g : β → γ → n (ForInStep γ)}
     {P : l} {Q : γ → l} {eQ : e}
@@ -1813,7 +1812,7 @@ theorem Spec.Iter.foldM_filterMapWithPostcondition {α β γ δ : Type w}
     {n : Type w → Type w'} {o : Type w → Type w''}
     {l : Type w} {e : Type w} [CompleteLattice l]
     [Iterator α Id β] [Finite α Id]
-    [Monad n] [Monad o] [LawfulMonad n] [LawfulMonad o] [WPMonad o l e]
+    [Monad n] [Monad o] [LawfulMonad n] [LawfulMonad o] [WP o l e]
     [IteratorLoop α Id n] [IteratorLoop α Id o]
     [LawfulIteratorLoop α Id n] [LawfulIteratorLoop α Id o]
     [MonadLiftT n o] [LawfulMonadLiftT n o]
@@ -1830,7 +1829,7 @@ theorem Spec.Iter.foldM_filterMapM {α β γ δ : Type w}
     {l : Type w} {e : Type w} [CompleteLattice l]
     [Iterator α Id β] [Finite α Id]
     [Monad n] [MonadAttach n] [LawfulMonad n] [WeaklyLawfulMonadAttach n]
-    [Monad o] [LawfulMonad o] [WPMonad o l e]
+    [Monad o] [LawfulMonad o] [WP o l e]
     [IteratorLoop α Id n] [IteratorLoop α Id o]
     [LawfulIteratorLoop α Id n] [LawfulIteratorLoop α Id o]
     [MonadLiftT n o] [LawfulMonadLiftT n o]
@@ -1846,7 +1845,7 @@ theorem Spec.Iter.foldM_mapWithPostcondition {α β γ δ : Type w}
     {m : Type w → Type w'''} {n : Type w → Type w'} {o : Type w → Type w''}
     {l : Type w} {e : Type w} [CompleteLattice l]
     [Iterator α Id β] [Finite α Id]
-    [Monad m] [Monad n] [Monad o] [LawfulMonad m] [LawfulMonad n] [LawfulMonad o] [WPMonad o l e]
+    [Monad m] [Monad n] [Monad o] [LawfulMonad m] [LawfulMonad n] [LawfulMonad o] [WP o l e]
     [IteratorLoop α Id n] [IteratorLoop α Id o]
     [LawfulIteratorLoop α Id n] [LawfulIteratorLoop α Id o]
     [MonadLiftT n o] [LawfulMonadLiftT n o]
@@ -1861,7 +1860,7 @@ theorem Spec.Iter.foldM_mapM {α β γ δ : Type w}
     {l : Type w} {e : Type w} [CompleteLattice l]
     [Iterator α Id β] [Finite α Id]
     [Monad n] [MonadAttach n] [LawfulMonad n] [WeaklyLawfulMonadAttach n]
-    [Monad o] [LawfulMonad o] [WPMonad o l e]
+    [Monad o] [LawfulMonad o] [WP o l e]
     [IteratorLoop α Id n] [IteratorLoop α Id o]
     [LawfulIteratorLoop α Id n] [LawfulIteratorLoop α Id o]
     [MonadLiftT n o] [LawfulMonadLiftT n o]
@@ -1875,7 +1874,7 @@ theorem Spec.Iter.foldM_filterWithPostcondition {α β δ : Type w}
     {n : Type w → Type w'} {o : Type w → Type w''}
     {l : Type w} {e : Type w} [CompleteLattice l]
     [Iterator α Id β] [Finite α Id]
-    [Monad n] [Monad o] [LawfulMonad n] [LawfulMonad o] [WPMonad o l e]
+    [Monad n] [Monad o] [LawfulMonad n] [LawfulMonad o] [WP o l e]
     [IteratorLoop α Id n] [IteratorLoop α Id o]
     [LawfulIteratorLoop α Id n] [LawfulIteratorLoop α Id o]
     [MonadLiftT n o] [LawfulMonadLiftT n o]
@@ -1890,7 +1889,7 @@ theorem Spec.Iter.foldM_filterM {α β δ : Type w}
     {l : Type w} {e : Type w} [CompleteLattice l]
     [Iterator α Id β] [Finite α Id]
     [Monad n] [MonadAttach n] [LawfulMonad n] [WeaklyLawfulMonadAttach n]
-    [Monad o] [LawfulMonad o] [WPMonad o l e]
+    [Monad o] [LawfulMonad o] [WP o l e]
     [IteratorLoop α Id n] [IteratorLoop α Id o]
     [LawfulIteratorLoop α Id n] [LawfulIteratorLoop α Id o]
     [MonadLiftT n o] [LawfulMonadLiftT n o]
@@ -1903,7 +1902,7 @@ theorem Spec.Iter.foldM_filterM {α β δ : Type w}
 theorem Spec.Iter.foldM_filterMap {α β γ δ : Type w}
     {n : Type w → Type w'}
     {l : Type w} {e : Type w} [CompleteLattice l]
-    [Iterator α Id β] [Finite α Id] [Monad n] [LawfulMonad n] [WPMonad n l e]
+    [Iterator α Id β] [Finite α Id] [Monad n] [LawfulMonad n] [WP n l e]
     [IteratorLoop α Id n]
     [LawfulIteratorLoop α Id n]
     {f : β → Option γ} {g : δ → γ → n δ} {init : δ} {it : Iter (α := α) β}
@@ -1917,7 +1916,7 @@ theorem Spec.Iter.foldM_filterMap {α β γ δ : Type w}
 theorem Spec.Iter.foldM_map {α β γ δ : Type w}
     {n : Type w → Type w'}
     {l : Type w} {e : Type w} [CompleteLattice l]
-    [Iterator α Id β] [Finite α Id] [Monad n] [LawfulMonad n] [WPMonad n l e]
+    [Iterator α Id β] [Finite α Id] [Monad n] [LawfulMonad n] [WP n l e]
     [IteratorLoop α Id n] [LawfulIteratorLoop α Id n]
     {f : β → γ} {g : δ → γ → n δ} {init : δ} {it : Iter (α := α) β}
     {P : l} {Q : δ → l} {eQ : e}
@@ -1928,7 +1927,7 @@ theorem Spec.Iter.foldM_map {α β γ δ : Type w}
 theorem Spec.Iter.foldM_filter {α β δ : Type w}
     {n : Type w → Type w'}
     {l : Type w} {e : Type w} [CompleteLattice l]
-    [Iterator α Id β] [Finite α Id] [Monad n] [LawfulMonad n] [WPMonad n l e]
+    [Iterator α Id β] [Finite α Id] [Monad n] [LawfulMonad n] [WP n l e]
     [IteratorLoop α Id n] [LawfulIteratorLoop α Id n]
     {f : β → Bool} {g : δ → β → n δ} {init : δ} {it : Iter (α := α) β}
     {P : l} {Q : δ → l} {eQ : e}
@@ -1940,7 +1939,7 @@ theorem Spec.Iter.fold_filterMapWithPostcondition {α β γ δ : Type w}
     {n : Type w → Type w'}
     {l : Type w} {e : Type w} [CompleteLattice l]
     [Iterator α Id β] [Finite α Id]
-    [Monad n] [LawfulMonad n] [WPMonad n l e]
+    [Monad n] [LawfulMonad n] [WP n l e]
     [IteratorLoop α Id n] [LawfulIteratorLoop α Id n]
     {f : β → PostconditionT n (Option γ)} {g : δ → γ → δ} {init : δ} {it : Iter (α := α) β}
     {P : l} {Q : δ → l} {eQ : e}
@@ -1954,7 +1953,7 @@ theorem Spec.Iter.fold_filterMapM {α β γ δ : Type w}
     {n : Type w → Type w'}
     {l : Type w} {e : Type w} [CompleteLattice l]
     [Iterator α Id β] [Finite α Id]
-    [Monad n] [MonadAttach n] [LawfulMonad n] [WeaklyLawfulMonadAttach n] [WPMonad n l e]
+    [Monad n] [MonadAttach n] [LawfulMonad n] [WeaklyLawfulMonadAttach n] [WP n l e]
     [IteratorLoop α Id n] [LawfulIteratorLoop α Id n]
     {f : β → n (Option γ)} {g : δ → γ → δ} {init : δ} {it : Iter (α := α) β}
     {P : l} {Q : δ → l} {eQ : e}
@@ -1968,7 +1967,7 @@ theorem Spec.Iter.fold_mapWithPostcondition {α β γ δ : Type w}
     {n : Type w → Type w'}
     {l : Type w} {e : Type w} [CompleteLattice l]
     [Iterator α Id β] [Finite α Id]
-    [Monad n] [LawfulMonad n] [WPMonad n l e]
+    [Monad n] [LawfulMonad n] [WP n l e]
     [IteratorLoop α Id n] [LawfulIteratorLoop α Id n]
     {f : β → PostconditionT n γ} {g : δ → γ → δ} {init : δ} {it : Iter (α := α) β}
     {P : l} {Q : δ → l} {eQ : e}
@@ -1980,7 +1979,7 @@ theorem Spec.Iter.fold_mapM {α β γ δ : Type w}
     {n : Type w → Type w'}
     {l : Type w} {e : Type w} [CompleteLattice l]
     [Iterator α Id β] [Finite α Id]
-    [Monad n] [MonadAttach n] [LawfulMonad n] [WeaklyLawfulMonadAttach n] [WPMonad n l e]
+    [Monad n] [MonadAttach n] [LawfulMonad n] [WeaklyLawfulMonadAttach n] [WP n l e]
     [IteratorLoop α Id n] [LawfulIteratorLoop α Id n]
     {f : β → n γ} {g : δ → γ → δ} {init : δ} {it : Iter (α := α) β}
     {P : l} {Q : δ → l} {eQ : e}
@@ -1992,7 +1991,7 @@ theorem Spec.Iter.fold_filterWithPostcondition {α β δ : Type w}
     {n : Type w → Type w'}
     {l : Type w} {e : Type w} [CompleteLattice l]
     [Iterator α Id β] [Finite α Id]
-    [Monad n] [LawfulMonad n] [WPMonad n l e]
+    [Monad n] [LawfulMonad n] [WP n l e]
     [IteratorLoop α Id n] [LawfulIteratorLoop α Id n]
     {f : β → PostconditionT n (ULift Bool)} {g : δ → β → δ} {init : δ} {it : Iter (α := α) β}
     {P : l} {Q : δ → l} {eQ : e}
@@ -2004,7 +2003,7 @@ theorem Spec.Iter.fold_filterM {α β δ : Type w}
     {n : Type w → Type w'}
     {l : Type w} {e : Type w} [CompleteLattice l]
     [Iterator α Id β] [Finite α Id]
-    [Monad n] [MonadAttach n] [LawfulMonad n] [WeaklyLawfulMonadAttach n] [WPMonad n l e]
+    [Monad n] [MonadAttach n] [LawfulMonad n] [WeaklyLawfulMonadAttach n] [WP n l e]
     [IteratorLoop α Id n] [LawfulIteratorLoop α Id n]
     {f : β → n (ULift Bool)} {g : δ → β → δ} {init : δ} {it : Iter (α := α) β}
     {P : l} {Q : δ → l} {eQ : e}
